\documentclass{article}
\usepackage[margin=1in]{geometry}
\usepackage{amsfonts}
\usepackage{amsmath}
\usepackage{amsthm}
\usepackage{parskip}
\usepackage{enumitem}

%\setlength{\parskip}{\baselineskip}
%\setlength{\parindent}{0pt}

\newtheorem*{lemma}{Lemma}

\begin{document}

\title{MTH 505 Homework 1}
\author{Roy Howie}
\date{February 1, 2017}
\maketitle

\section{Developing $\mathbb{N}$}
Completed in the following order: a, b, c, d, e, h, f, g.
\begin{enumerate}[label=\textbf{(\alph*)}]
\item{
	Let
	$S=\{ n \in \mathbb{N} \mid n = 0 \ \vee \
		\exists m \in \mathbb{N} \text{ such that } \sigma(m)=n
	\}$.
	Note $0 \in S$.
	Next, suppose $x \in S$, then $\sigma(x) \in S$, as
	there exists $m \in \mathbb{N}$ such that
	$\sigma(m) = \sigma(x)$: namely, $x$ itself.
	Hence, $\bf{P4}$
	$\Rightarrow S = \mathbb{N}$.

	Next, fix $n \in \mathbb{N}$ and suppose
	$\exists m_1,m_2 \in \mathbb{N}$ such that
	$\sigma(m_1) = n = \sigma(m_2)$ and $m \ne n$.
	This is a contradiction.
	By $\bf{P3}$, $\sigma(m_1)=\sigma(m_2)$ implies $m_1=m_2$.
	Hence, predecessors are unique.
	\hfill $\square$
}

\item{
	Fix $a,b \in \mathbb{N}$ and let
	$S=\{ c \in \mathbb{N} \mid a+(b+c)=(a+b)+c \}$.
	By $\bf{(1)}$, $0 \in S$ as
	$a+(b+0) = a+(b) = (a+b) + 0$.
	Next, suppose $n \in S$, then
	\begin{align*}
		a+(b+\sigma(n))&= a+\sigma(b+n)		\tag{2} \\
                       &= \sigma(a+(b+n))	\tag{2} \\
                       &= \sigma((a+b)+n)	\tag{IH}\\
                       &= (a+b) + \sigma(n) \tag{2}
	\end{align*}
	Hence, $\sigma(n) \in S$, so $\bf{P4}$
	$\Rightarrow S = \mathbb{N}$.
	\hfill $\square$
}
\item{
	Let $S = \{ n \in \mathbb{N} \mid 0 + n = n \}$.
	By $\bf{(1)}$, $0 \in S$ as $0+0=0$.
	Next, suppose $x \in S$, then
	\begin{align*}
		0 + \sigma(x) &= \sigma(0 + x)	\tag{2} \\
					  &= \sigma(x)		\tag{IH}
	\end{align*}
	Hence, $\sigma(x) \in S$, so $\bf{P4}$
	$\Rightarrow S = \mathbb{N}$. In addition,
	via $\bf{(1)}$, one has
	$ 0 + n = n + 0$ for all $n \in \mathbb{N}$.
	
	Let
	$ R = \{ n \in \mathbb{N} \mid
		n+\sigma(0) = \sigma(0) + n \}
	$. By above, $0 \in R$, as
	$ 0 + \sigma(0) = \sigma(0) + 0$.
	Suppose $x \in R$, then
	\begin{align*}
		\sigma(x)+\sigma(0) &= \sigma(\sigma(x) + 0)	\tag{2} \\
		  &= \sigma(\sigma(x))			\tag{1} \\
		  &= \sigma(\sigma(x+0))		\tag{1} \\
		  &= \sigma(x+\sigma(0))		\tag{2} \\
		  &= \sigma(\sigma(0)+x)		\tag{IH} \\
		  &= \sigma(0) + \sigma(x)		\tag{2}
	\end{align*}
	Hence, $\sigma(x) \in R$, so $\bf{P4}$
	$\Rightarrow R = \mathbb{N}$.
	\hfill $\square$
}
\item{
	Fix $a \in \mathbb{N}$ and let
	$S=\{b \in \mathbb{N} \mid a+b=b+a \}$.
	By $\bf{(c)}$, $0 \in S$.
	Suppose $x \in S$, then
	\begin{align*}
		a+\sigma(x) &= \sigma(a+x)		\tag{2} \\
					&= \sigma(x+a)		\tag{IH}\\
					&= \sigma((x+a)+0)	\tag{1} \\
					&= (x+a)+\sigma(0)	\tag{2} \\
					&= x+(a+\sigma(0))	\tag{b} \\
					&= x+(\sigma(0)+a)	\tag{c} \\
					&= (x+\sigma(0))+a	\tag{b} \\
					&= \sigma(x+0)+a	\tag{2} \\
					&= \sigma(x)+a		\tag{1}
	\end{align*}
	Hence, $\sigma(x) \in S$, so $\bf{P4}$
	$\Rightarrow S = \mathbb{N}$.
	\hfill $\square$
}
\item{
	Fix $b,c \in \mathbb{N}$ and let
	$S=\{ a \in \mathbb{N} \mid (b+c)a = ba + ca \}$.
	By $\bf{(1)}$ and $\bf{(3)}$, $0 \in S$, as
	$(b+c)*0 = 0 + 0$.
	Suppose $x \in S$, then
	\begin{align*}
		(b+c)\sigma(x) &= (b+c)x+(b+c)	\tag{4} \\
			&= (bx+cx)+(b+c)			\tag{IH}\\
			&= (bx+b)+(cx+c)			\tag{b,d}\\
			&= b\sigma(x)+c\sigma(x)	\tag{4}
	\end{align*}
	Hence, $\sigma(x) \in S$, so $\bf{P4}$
	$\Rightarrow S = \mathbb{N}$.
	\hfill $\square$
}
\item{
	Fix $a,b \in \mathbb{N}$ and let
	$S=\{c \in \mathbb{N} \mid (ab)c=a(bc) \}$.
	By $\bf{(3)}$, $0 \in S$, as
	$a(b*0)=0=(ab)*0$.
	Suppose $x \in S$, then
	\begin{align*}
		a(b\sigma(x)) &= a(bx+b) 		\tag{4}\\
			&= a(bx) + ab				\tag{h,e}\\
			&= (ab)x + ab				\tag{IH}\\
			&= (ab)x + ab\sigma(0)		\tag{h}\\
			&= (ab)(x+\sigma(0))		\tag{e}\\
			&= (ab)\sigma(x+0)			\tag{2}\\
			&= (ab)\sigma(x)			\tag{1}
	\end{align*}
	Hence, $\sigma(x) \in S$, so $\bf{P4}$
	$\Rightarrow S = \mathbb{N}$.
	\hfill $\square$
}
\item{
	By $\bf{(h)}$ and $\bf{(4)}$,
	$\sigma(a)b=b\sigma(a)=ba+b=ab+b$.
	\hfill $\square$
}
\item{
	Let $S=\{n\in\mathbb{N}\mid0*a=0\}$.
	By $\bf{(3)}$, $0 \in S$, as
	$0*0=0$.
	Suppose $x\in S$, then
	\begin{align*}
		0*\sigma(x) &= 0*x + 0	\tag{4} \\
			&= 0 + 0			\tag{IH}\\
			&= 0				\tag{1}
	\end{align*}
	Hence, $\sigma(x) \in S$, so $\bf{P4}$
	$\Rightarrow S = \mathbb{N}$.

	Let $R=\{a\in\mathbb{N}\mid \sigma(0)*a=a\}$.
	By $\bf{(1)}$, $0 \in S$, as
	$\sigma(0)*0=0$.
	Suppose $x \in S$, then
	\begin{align*}
		\sigma(0)\sigma(x) &= \sigma(0)x+\sigma(0)	\tag{4}\\
			&= x + \sigma(0)		\tag{IH}\\
			&= \sigma(x+0)			\tag{2} \\
			&= \sigma(x)			\tag{1}
	\end{align*}
	Hence, $\sigma(x) \in R$, so $\bf{P4}$
	$\Rightarrow R = \mathbb{N}$.
	
	Fix $a\in\mathbb{N}$ and let
	$Q=\{b\in\mathbb{N}\mid ab=ba\}$.
	By above, $0 \in Q$ because $0*a=a*0$.
	Suppose $x\in Q$, then
	\begin{align*}
		a\sigma(x) &= ax+a		\tag{4} \\
			&= xa+a				\tag{IH}\\
			&= xa+\sigma(0)a	\tag{above}\\
			&= (x+\sigma(0))a	\tag{e}\\
			&= \sigma(x+0)a		\tag{2}\\
			&= \sigma(x)a		\tag{1}
	\end{align*}
	Hence, $\sigma(x) \in Q$, so $\bf{P4}$
	$\Rightarrow Q = \mathbb{N}$.
	\hfill $\square$
}
\end{enumerate} 
  
\hfill\break
\begin{lemma}{(Additive Cancellation)}
	For $a,b,c \in \mathbb{N}$, if $a+c=b+c$, then $a=b$.
\end{lemma}
\begin{proof}
	Fix $a,b\in\mathbb{N}$ and let
  	$S=\{c\in\mathbb{N}\mid a+c=b+c\Rightarrow a=b\}$.
  	Note $0\in S$. Suppose $x\in S$, then
  	\begin{align*}
    	a+\sigma(x) &= b+\sigma(x)          \\
    	\sigma(a+x) &= \sigma(b+x) \tag{2}  \\
                a+x &= b+x         \tag{P3} \\
                  a &= b           \tag{IH}
  \end{align*}
  Hence $\sigma(x) \in S$, so $\bf{P4}$
  $\Rightarrow S = \mathbb{N}$.
\end{proof}


\section{From $\mathbb{N}$ to $\mathbb{Z}$}
\begin{enumerate}[label=\textbf{(\alph*)}]
\item{
	To show $[a,b] \sim [c,d] \iff a+d=c+b$
	is an equivalence relation:
	\begin{enumerate}[label=(\arabic*)]
	\item{
		$[a,b] \sim [a,b] \Rightarrow a+b=a+b$
	}
	\item{
		$[a,b] \sim [c,d] \Leftrightarrow [c,d] \sim [a,b]$.
		Note that
		$[a,b]\sim[c,d]
			\Leftrightarrow a+d=c+b
			\Leftrightarrow c+b=a+d
			\Leftrightarrow [c,d]\sim[a,b]
		$.
	}
	\item{
		$[a,b]\sim[c,d]\wedge[c,d]\sim[e,f]\Rightarrow[a,b]\sim[e,f]$.
		By assumption, $a+d=b+c$ and $c+f=e+d$.
		\begin{align*}
			a+d &= c+b        \\
			(a+d)+f&=(c+b)+f  \\
			       &= b+(c+f)  \\
			       &= b+(e+d)  \\
			       &= (e+b)+d  \\
		   (a+f)+d &=(e+b)+d
		\end{align*}
		Hence, by the Additive Cancellation Lemma, $a+f=e+b$, so
		$[a,b]\sim[e,f]$.
		\hfill $\square$
	}
	\end{enumerate}
}
\item{
	\begin{enumerate}[label=(\arabic*)]
	\item{
		To show $[a,b]+[c,d]=[a+c,b+d]$ is well-defined,
		consider $[a,b]\sim[a',b']$ and
		$[c,d]\sim[c',d']$.
		Note that $a+b'=a'+b$ and $c+d'=c'+d$.
		Therefore,
		$(a+b')+(c+d')=(a'+b)+(c'+d)$.
		Some shuffling of terms yields
		$(a+c)+(b'+d')=(a'+c')+(b+d)$,
		implying
		$[a+c,b+d]\sim[a'+c',b'+d']$,
		so addition on equivalence classes is indeed
		well-defined.
	}
	\item{
		To show $[a,b]*[c,d]=[ac+bd,ad+bc]$ is well-defined,
		again consider $[a,b]\sim[a',b']$ and
		$[c,d]\sim[c',d']$.
		
		We want
		$[ac+bd,ad+bc]\sim[a'c'+b'd',a'd'+b'c']$,
		or $(ac+bd)+(a'd'+b'c')=(a'c'+b'd')+(ad+bc)$.
		We have $a+b'=a'+b$ and $c+d'=c'+d$.
		We only need imagination:
		\begin{align*}
			(a+b')+(a'+b)+(c+d')+(c'+d) &= (a'+b)+(a+b')+(c'+d)+(c+d') \\
            (a+b')c+(a'+b)d+(c+d')a'+(c'+d)b'
           	     &= (a'+b)c+(a+b')d+(c'+d)a'+(c+d')b' \\
			(ac+b'c)+(a'd+bd)+(ca'+d'a')+(c'b'+db')
			     &= (a'c+bc)+(ad+b'd)+(c'a'+da')+ (cb'+d'b') \\
			(ac+bd)+(d'a'+c'b')+(b'c+a'd+ca'+db')
			 	 &= (c'a'+d'b')+(ad+bc)+(a'c+b'd+da'+cb') \\
		    (ac+bd)+(d'a'+c'b') &= (c'a'+d'b')+(ad+bc)
		\end{align*}
		The general rule is to keep numbers of the form
		$ab$ or $a'b'$ but not $a'b$ or $ab'$.
		Nevertheless, the last line implies the desired result,
		so multiplication on equivalence classes is
		well-defined.
		\hfill $\square$
	}
	\end{enumerate}
}
\item{
	\begin{enumerate}[label=(\arabic*)]
	\item{
		Associativity of $+:\mathbb{Z}\to\mathbb{Z}$
		\begin{align*}
			([a,b]+[c,d])+[e,f] &= [a+c,b+d]+[e,f]\\
				&= [(a+c)+e,(b+d)+f]\\
				&= [a+(c+e),b+(d+f)]\\
				&= [a,b]+[c+e,d+f]\\
				&= [a,b]+([c,d]+[e,f])
		\end{align*}
	}
	\item{
		Commutativity of $+:\mathbb{Z}\to\mathbb{Z}$
		\begin{align*}
			[a,b]+[c,d] &= [a+c,b+d]\\
				&=[c+a,d+b]\\
				&=[c,d]+[a,b]
		\end{align*}
	}
	\item{
		Associativity of $*:\mathbb{Z}\to\mathbb{Z}$
		\begin{align*}
			([a,b]*[c,d])*[e,f] &= [ac+bd,ad+bc]*[e,f]\\
				&= [(ac+bd)e+(ad+bc)f,(ac+bd)f+(ad+bc)e]\\
				&= [ace+bde+adf+bcf,acf+bdf+ade+bce]\\
				&= [a(ce+df)+b(cf+de),a(cf+de)+b(df+ce)]\\
				&= [a,b]*[ce+df,cf+de]\\
				&= [a,b]*([c,d]*[e,f])
		\end{align*}
	}
	\item{
		Commutativity of $*:\mathbb{Z}\to\mathbb{Z}$
		\begin{align*}
			[a,b]*[c,d] &= [ac+bd,ad+bc] \\
				&= [ca+db,cb+da] \\
				&= [c,d]*[a,b]
		\end{align*}
	}
	\hfill $\square$
	\end{enumerate}
}
\item{
	First, additive inverses are added, which turns
	$\mathbb{N}$ into an abelian group $\mathbb{Z}'$.
	Next, a second binary operation, multiplication, is
	added to transform the abelian group
	$\mathbb{Z}'$ into the commutative ring $\mathbb{Z}$.
	Every $n\in\mathbb{N}$ has an ``additive inverse''
	in the form of the members of the equivalence class of $[0,n]$.
}
\end{enumerate}

\vfill
\section{From $\mathbb{Z}$ to $\mathbb{Q}$}
\begin{enumerate}[label=\textbf{(\alph*)}]
\item{
	To show $[a,b]\sim[c,d] \Leftrightarrow ad=bc$
	is an equivalence relation:
	\begin{enumerate}[label=(\arabic*)]
	\item{
		$[a,b]\sim[a,b] \Rightarrow ab=ba$
	}
	\item{
		$[a,b]\sim[c,d]\Leftrightarrow[c,d]\sim[a,b]$
		Note that
		$[a,b]\sim[c,d]
			\Rightarrow ad = bc
			\Rightarrow cb = da
			\Rightarrow [c,d]\sim[a,b]
		$.
	}
	\item{
		$[a,b]\sim[c,d]\wedge[c,d]\sim[e,f]\Rightarrow[a,b]\sim[e,f]$.
		By assumption, $ad=bc$ and $cf=de$.
		\begin{align*}
			(ad)f &= (bc)f \\
				  &= b(cf) \\
			      &= b(de) \\
			 (af)d&= (be)d
		\end{align*}
		Hence, by multiplicative cancellation,
		$af=be$, so $[a,b]\sim[e,f]$.
		\hfill $\square$
	}
	\end{enumerate}
}
\item{
	\begin{enumerate}[label=(\arabic*)]
	\item{
		To show $[a,b]*[c,d]=[ac,bd]$ is well-defined, consider
		$[a,b]\sim[a',b']$ and $[c,d]\sim[c',d']$.
		Note that $ab'=ba'$ and $cd'=dc'$.
		Therefore, $(ab')(cd')=(ba')(dc')$.
		Shuffling terms gives $(ac)(b'd')=(bd)(a'c')$,
		implying $[ac,bd]\sim[a'c',b'd']$.
		Hence, multiplication is well-defined.
	}
	\item{
		To show $[a,b]+[c,d]=[ad+bc,bd]$ is well-defined, again consider
		$[a,b]\sim[a',b']$ and $[c,d]\sim[c',d']$.
		\begin{align*}
			(ab')+(cd') &= (ba')+(dc')\\
			(bb'+dd')(ab'+cd') &= (ba'+dc')(dd'+bb')\\
			(ab'dd'+cd'bb')+(ab'bb'+cd'dd')
				&= (a'bdd'+c'dbb')+(ba'bb'+dc'dd')\\
			ab'dd'+cd'bb' &= a'bdd'+c'dbb'\\
			(ad)(b'd')+(bc)(b'd')
				&= (a'd')(bd)+(b'c')(bd)\\
			(ad+bc)(b'd')&=(bd)(a'd'+b'c')
		\end{align*}
		Hence, $[ad+bc,bd]\sim[a'd'+b'c',b'd']$ and
		addition is well-defined.
	}
	\hfill $\square$
	\end{enumerate}
}
\item{
	Too tedious.
}
\item{
	$\mathbb{Z}$ is a commutative ring, whereas
	$\mathbb{Q}$ is a field. Thus, to transition from
	$\mathbb{Z}$ to $\mathbb{Q}$, one needs
	multiplicative inverses for all nonzero integers.
	Thus, every $q\in\mathbb{Q}$ is represented by an
	equivalence class $[a,b]$ and has a corresponding
	``multiplicative inverse'' represented by the
	equivalence class $[b,a]$.
}
\end{enumerate}
\end{document}














